
\section{Fibonacci proof using induction}\label{induction_proof}

The Fibonacci sequence is defined as:
\begin{align}
	&F_i = F_{i-1} + F_{i-2} \hspace{10mm} \text{for} \hspace{5 mm} i \geq 2\\
	&F_1 = 1 , F_2 = 1
\end{align}
We want to prove that:

\begin{equation}
\sum\limits_{i=1}^n F_i = F_{n+2} - 1
\end{equation}

\textbf{Basis step:}

We want to show that our statement holds for the smallest i, namely i = 2:
\begin{align}
F_1 + F_2 &\stackrel{?}{=} F_{2 + 2} - 1 = F_4 - 1\\
F_1 + F_2 &\stackrel{?}{=} (F_3 + F_2) -1\\
F_1 + F_2 &\stackrel{?}{=} ((F_2 + F_2) + F_2) - 1\\
F_1 + F_2 &\stackrel{?}{=} 1 + 1 + 1 -1 \\
2 &= 2\\
\end{align}
\textbf{Induction step:}
Now that we have shown that the statement holds for n, we want to show that the statement holds for $n+1$, by replacing $n$ with $n+1$:
\begin{align}
\sum\limits_{i=1}^{n+1} F_{i} &\stackrel{?}{=} F_{(n + 1)+2} - 1\\
F_1 + F_2 + F_3 + ... + F_n + F_{n+1} &\stackrel{?}{=} F_{n + 3} -1\\
F_1 + F_2 + F_3 + ... + F_n + F_{n+1} &\stackrel{?}{=} F_{n + 2} + F_{n + 1} -1\\
\left(\sum\limits_{i=1}^n F_{i} \right) + F_{n+1} &\stackrel{?}{=} F_{n + 2} + F_{n + 1} -1\\
\intertext{Now, we can use what we have proven in the basis step, to reduce this:}
\left( \sum\limits_{i=1}^n F_{i} \right) + F_{n+1} &\stackrel{?}{=} F_{n + 2} + F_{n + 1} -1\\
F_{n+1} &= F_{n + 1}
\end{align}
\hspace{120mm} $Q.E.D$\\\\
Since this is true, the original statement must therefore also be true, and the proof is complete.
